\documentclass{article}
\usepackage[utf8]{inputenc}
\usepackage[english]{babel}
\usepackage[]{amsthm}
\usepackage[]{amssymb}
\usepackage[]{amsmath}
\usepackage[]{graphicx}
\usepackage[]{hyperref}
\usepackage[]{xcolor}
\usepackage[]{cancel}
\usepackage[]{fancyhdr}
\hypersetup{
    colorlinks,
    linkcolor={red!50!black},
    citecolor={blue!50!black},
    urlcolor={blue!80!black}
}

\pagestyle{fancy}
\fancyhf{}
\title{\vspace{-4cm}MTH20012 - Series and Transformations Test 3}
\author{Joshua Rogers}
\lhead{MTH20012 Test 3}
\rhead{Joshua Rogers 101096819}
\date\today

\begin{document}
\maketitle 

\section*{Part C, Question 5}
\subsection*{Part A}
Use Laplace transforms to obtain the soutions of the following system of differential equations:

$$
\frac{dx}{dt} = x^{'} = -6x+y
$$
$$
\frac{dy}{dt} = y^{'} = 4x-3y
$$

given $x(0) = -3$ and $y(0) =-4$.
\subsubsection*{Answer}

\[ \begin{cases}
sX(s)-x(0)=-6X(s)+Y(s) \\
sY(s)-y(0) = 4X(s)-3Y(s)
   \end{cases}
\]

\[ \begin{cases}
sX(s)+3=-6X(s)+Y(s) \\
sY(s)+4 = 4X(s)-3Y(s)
   \end{cases}
\]

Letting $X(s)=x$ and $Y(s)=y$ for the moment we obtain the simultaneous equations
\[ \begin{cases}
sx+3=-6x+y \\
sy+4 = 4x-3y
   \end{cases}
\]

substituting $y=sx+6x+3$ into $sy+4=4x-3y$ we obtain

$$s(sx+6x+3)+4=4x-3(sx+6x+3)$$
$$s^2x+6sx+3s+4=-3sx-14x-9$$
$$x\left[s^2+9s+14\right]=-3s-13$$

Thus, we have

$$X(s) = -\frac{3s+13}{s^2+9s+14} = -\frac{1}{5} \left[ \frac{8}{s+7}+\frac{7}{s+2}\right]$$
Using the reverse shift theorem we thus have

$$\mathcal{L}^{-1}\left\{\frac{1}{s+2}\right\} = e^{-2t}$$
and
$$\mathcal{L}^{-1}\left\{\frac{1}{s+7}\right\} = e^{-7t}$$

thus we have

$$x(t) = -\frac{1}{5} \left[ 7e^{-2t}+8e^{-7t}\right]$$

Likewise, we have

$$sX(s)+3+6X(s)=Y(s)$$
or
$$sx+3+6x=y$$

$$y=3-\frac{s\left(3s+13\right)}{s^2+9s+14} -\frac{6\left(3s+13\right)}{s^2+9s+14} = - \frac{4\left(s+9\right)}{(s+7)(s+2)} = \frac{8}{5(s+7)}-\frac{28}{5(s+2)}$$

Once again using the reverse shift theorem exactly as before, we obtain

$$y(t) = -\frac{4}{5} \left[ 7e^{-2t}-2e^{-7t} \right]$$


Thus we have obtained

\[ \begin{cases}
x(t) = -\frac{1}{5} \left[ 7e^{-2t}+8e^{-7t}\right] \\
y(t) = -\frac{4}{5} \left[ 7e^{-2t}-2e^{-7t} \right]
\end{cases}
\]
\subsection*{Part B}
Verify the solution satisfies the differential equations.
\subsubsection*{Answer}

$$x(0) = -\frac{1}{5} \left[ 7+8 \right] = -3$$
$$y(0) = -\frac{4}{5} \left [ 7-2 \right] = -4$$

Likewise, we have
\[ \begin{cases}
x^{'}(t) = \frac{14}{5} \left[ e^{-2t}+4e^{-7t} \right] \\
y^{'}(t) = \frac{14}{5} \left[ e^{-2t}+4e^{-7t} \right]
\end{cases}
\]

Putting this into the original system of differential equations, obtain

$$  \frac{14}{5} \left[ e^{-2t}+4e^{-7t} \right] = -6 \left[ -\frac{1}{5} \left[ 7e^{-2t}+8e^{-7t}\right] \right ] +  -\frac{4}{5} \left[ 7e^{-2t}-2e^{-7t} \right]$$

$$ 56e^{-7t}+14e^{-2t}=48e^{-7t}+42e^{-2t}-28e^{-2t}+8e^{-7t} $$

$$56e^{-7t}+14e^{-2t}=48e^{-7t}+42e^{-2t}-28e^{-2t}+8e^{-7t}$$

RHS = LHS, thus this is true and the solutions are valid.

\end{document}
