\documentclass{article}
\usepackage[utf8]{inputenc}
\usepackage[english]{babel}
\usepackage[]{amsthm}
\usepackage[]{amssymb}
\usepackage[]{amsmath}
\usepackage[]{hyperref}
\usepackage[]{xcolor}
\usepackage[]{cancel}
\usepackage[]{fancyhdr}
\hypersetup{
    colorlinks,
    linkcolor={red!50!black},
    citecolor={blue!50!black},
    urlcolor={blue!80!black}
}

\pagestyle{fancy}
\fancyhf{}
\title{\vspace{-4cm}MTH20012 - Series and Transformations Test 1}
\author{Joshua Rogers}
\lhead{MTH20012 Test 1}
\rhead{Joshua Rogers 101096819}
\date\today

\begin{document}
\maketitle 

\section*{Part A}
\subsection*{One - Three}

Determine the limit of the following equations.

\begin{equation}\label{a1}
\lim_{n\to\infty} \frac{11+2n+2n^3}{-4-2n+10n^2+5n^3}
\end{equation}
\begin{equation}\label{a2}
\lim_{n\to\infty} \frac{3n!+3n^n}{n^2-3(2^n)}
\end{equation}
\begin{equation}\label{a3}
\lim_{n\to\infty} \sqrt{5n+2\sqrt{n}}-\sqrt{5n+3\sqrt{n}}
\end{equation}


\subsubsection*{Answers}

For \ref{a1}:
\begin{align*}
&\lim_{n\to\infty} \frac {11-2n-2n^3}{-4-2n+10n^2+5n^3}\\
&\lim_{n\to\infty} \frac{ \cancel{n^3} \left(\cancelto{0}{\frac{11}{n^3}}\cancelto{0}{-\frac{2}{n^2}}-2\right)}{\cancel{n^3} \left(\cancelto{0}{\frac{-4}{n^3}}-\cancelto{0}{\frac{2}{n^2}}+\cancelto{0}{\frac{10}{n}}+5\right)} n \rightarrow \infty = \frac{-2}{5}
\end{align*}
\par

\subsection*{}

For \ref{a2}:

Rewriting the formula, we obtain

\[
\frac{3n!}{-3 \cdot 2^n + n^2} + \frac{3n^n}{-3 \cdot 2^n + n^2}
\]

For the first term we have
\[
\left|\frac{3n!}{n^2-3 \cdot 2^n}\right| \geq \left| \frac{3n!}{-3 \cdot 2^n} \right| = \left|\frac{n!}{2^n}\right| \rightarrow \infty
\]

Since $n^2-3 \cdot 2^n < 0$ for $n \geq 5$, the equation must go to $- \infty$.

For the second term, we note that $n^n >0$ and $n^2 - 3 \cdot 2^n < 0$ , and thus must go towards $-\infty$.

Thus, we have shown that the limit is $-\infty$.


\par
\subsection*{}

For \ref{a3}:

Rationializing the equation yields

\begin{align*}
\frac{(\sqrt{5n+2\sqrt{n}}-\sqrt{5n+2\sqrt{n}})(\sqrt{5n+2\sqrt{n}}+\sqrt{5n+3\sqrt{n}}} {\sqrt{5n+2\sqrt{n}}+\sqrt{5n+3\sqrt{n}}} \Bigr| (a-b)(a+b)=a^2-b^2\\
= \frac{-\sqrt{n}}{\sqrt{5n+2\sqrt{n}}+\sqrt{5n+3\sqrt{n}}}
\end{align*}

Multiplying the denominator and the numberator by $\frac{1}{\sqrt{n}}$ yields

\begin{align*}
\frac{\frac{1}{\sqrt{n}} \cdot \sqrt{n}}{ \frac{1}{\sqrt{n}}\left(\sqrt{5n+2\sqrt{n}}+\sqrt{5n+3\sqrt{n}}\right)} = \frac{1}{ \sqrt{5+\frac{2}{\sqrt{n}}}+\sqrt{5+\frac{3}{\sqrt{n}}}}\\
\lim_{n\to\infty} \frac{1}{ \sqrt{5+\cancelto{0}{\frac{2}{\sqrt{n}}}}+\sqrt{5+\cancelto{0}{\frac{3}{\sqrt{n}}}}}\\\\
\therefore \lim_{n\to\infty} \ref{a3} = \frac{-1}{2\sqrt{5}}
\end{align*}
\par

\subsection*{Four}

Determine whether the following series converges and if so, find its sum.

\begin{equation}\label{a4}
\sum_{n=0}^{\infty} \frac {(-1)^n3^{n-4}4^{n+3}}{5^{2n-1}}
\end{equation}

\subsubsection*{Answers}

Rewriting the sum,
\[
a_n = \frac{ (-1)^n \cdot 3^n \cdot 4^3 \cdot 4^n \cdot 5}{3^4 \cdot 5^{2n}}
\]

Performing the root test.
\begin{align*}
L = \lim_{n\to\infty} & \left| \left( \frac{(-1)^n \cdot 3^n \cdot 4^3 \cdot 4^n \cdot 5} {3^4 \cdot 5^{2n}}\right)^{\frac{1}{n}}\right| \\
& \left |\frac{-1 \cdot 3 \cdot 4^{\frac{3}{n}} \cdot 4 \cdot 5^{\frac{1}{n}}}{3^{\frac{1}{n}} \cdot 5^2} \right| \\
& \left | \frac {12 \cdot \cancelto{1}{4^{\frac{3}{n}}} \cdot \cancelto{1}{5^{\frac{1}{n}}}}{25 \cdot \cancelto{1}{3^{\frac{1}{n}}}} \right | \rightarrow n \to \infty.
\end{align*}
The series therefore absolutely conveges;  $\frac{12}{25} < 1$.

To determine the sum:
\begin{align*}
\frac{ (-1)^n \cdot 3^n \cdot 4^3 \cdot 4^n \cdot 5}{3^4 \cdot 5^{2n}}
= \left(\frac{-12}{25}\right)^n \cdot \frac{4^3 \cdot 5}{3^4} = \frac{320}{81} \cdot \left(\frac{-12}{25}\right)^n
\end{align*}
\[
S = \frac{320}{81} \cdot \frac{1}{1-\left(\frac{-12}{25}\right)} = \frac{8000}{2997}
\]

\par

\subsection*{Five}
Expand the following series and provide a numerical value for the sum that is correct to 6 decimal places.

\begin{equation}\label{a5}
\sum_{k=3}^{5} \frac{(-1)^k\ln{4k}}{3k^2+17}
\end{equation}

\subsubsection*{Answers}

For k=3,4,5, we obtain:
\[
\frac{(-1)^3\ln{12}}{3\cdot 3^2+17} + \frac{(-1)^4\ln{16}}{3\cdot 4^2+17} + \frac{(-1)^5\ln{20}}{3\cdot 5^2+17} = 0.046382
\]

\par

\subsection*{Six}

Determine the convergence of the following equation.
\begin{equation}\label{a6}
\sum_{n=1}^{\infty} \frac{5n^2+2}{4n^2+4n+13}
\end{equation}

\subsubsection*{Answers}

Using the limit test, we check whether the limit of $a_n$ exists. If it does, it is clear that it is impossible for the series to converge.

\begin{align*}
\lim_{n\to\infty} \frac{5n^2+2}{4n^2+4n+13} = \lim_{n\to\infty} \frac{ \cancel{n^2}\left(5+\cancelto{0}{\frac{2}{n^2}}\right)}{\cancel{n^2}\left(4+\cancelto{0}{\frac{4}{n}}+\cancelto{0}{\frac{13}{n^2}}\right)} = \frac{5}{4}.
\end{align*}

Given that $\lim_{n\to\infty} \ref{a6} \neq 0$, the series diverges.
\par

\end{document}
