\documentclass{article}
\usepackage[utf8]{inputenc}
\usepackage[english]{babel}
\usepackage[]{amsthm}
\usepackage[]{amssymb}
\usepackage[]{amsmath}
\usepackage[]{graphicx}
\usepackage[]{hyperref}
\usepackage[]{xcolor}
\usepackage[]{cancel}
\usepackage[]{fancyhdr}
\hypersetup{
    colorlinks,
    linkcolor={red!50!black},
    citecolor={blue!50!black},
    urlcolor={blue!80!black}
}

\pagestyle{fancy}
\fancyhf{}
\title{\vspace{-4cm}MTH20012 - Series and Transformations Test 3}
\author{Joshua Rogers}
\lhead{MTH20012 Test 3}
\rhead{Joshua Rogers 101096819}
\date\today

\begin{document}
\maketitle 

\section*{Part B, Question 4}
\begin{align*}
12x^{''}+48x=3\sin(2t) && x(0)=0, x^{'}(0)=0
\end{align*}

\subsection*{Part A}
Find the expression for $X(s)$.
\subsubsection*{Answer}

$$12 \left(s^2X(s)-sx(0)-x^{'}(0)\right) + 48 X(s)=\frac{6}{s^2+4}$$

$$12s^2X(s)+48X(s)=\frac{6}{s^2+4}$$
$$X(s) \left[ 12s^2 + 48 \right] = \frac{6}{s^2+4}$$
$$X(s) = \frac{6}{(s^2+4)(12s^2+48)} = \frac{1}{2\left(s^2+4\right)^2}$$

\subsection*{Part B}
Find the laplace transform of
$$f(t) = 2t \cos(2t) - \sin(2t)$$
\subsubsection*{Answer}
Using linearity we solve $\mathcal{L}\{2t cos(2t)\} - \mathcal{L}\{sin(2t)\}$
Using the first shift theorem, convolution theorem, the standard laplace transforms of sin and cos, we obtain

$$F(s) = \frac{2(s^2-4)}{(s^2+4)^2} - \frac{2}{s^2+4} = -\frac{16}{(s^2+4)^2}$$

\pagebreak
\subsection*{Part C}
Express $X(s)$ in terms of $F(s)$.
\subsubsection*{Answer}

\begin{align*}
X(s) = \frac{1}{2\left(s^2+4\right)^2} && F(s) = -\frac{16}{(s^2+4)^2}
\end{align*}

$$
\frac{1}{2\cancel{\left(s^2+4\right)^2}} = A \cdot -\frac{16}{\cancel{(s^2+4)^2}}
$$

Given $A=-\frac{1}{32}$, we thus have

$$X(s) = -\frac{1}{32} F(s)$$

\subsection*{Part D}
Find $x(t)$.
\subsubsection*{Answer}
We have
$$X(s) = -\frac{1}{32} F(s)$$

$$\mathcal{L}^{-1}\{X(s)\} = x(s) = -\frac{1}{32} \mathcal{L}^{-1}\{F(s)\} = -\frac{1}{32} f(t)$$

Thus we have, by using the information provided

$$
x(t) = \frac{1}{32} \left( \sin(2t) - 2t\cos(2t)\right)
$$

\subsection*{Part E}
Verify the solution using the initial value conditions.
\subsubsection*{Answer}

We have
$$x(0) = \frac{1}{32} \left( \sin(2 \cdot 0) - 2\cdot 0 \cos(2\cdot 0)\right) = 0$$
as expected.

$$x^{'}(t) = \frac{1}{32} \left[2\cos(2t)+4t\sin(2t)-2\cos(2t)\right] = \frac{1}{8}t \sin(2t)$$
thus
$$x^{'}(0) = 0$$
as expected. 
\end{document}
